A lot of examples work with tactics

iodiv/IODiv.fst
@@ -1102,11 +1102,25 @@ let test_2 (s : string) : IODiv file_descr (requires True) (ensures fun _ -> Tru
   let msg = test_1 s in
   open_file s
 
-// Sadly the following fails... because of a failed subcomp it seems.
-// let test (s : string) : IODiv unit (requires True) (ensures fun _ -> True) = // (ensures fun r -> terminates r /\ (exists fd msg. ret_trace r == [ Call_choice #cmds #io_op_sig Openfile s fd ; Call_choice Read fd msg ; Call_choice Close fd () ])) =
-//   let fd = open_file s in
-//   let msg = read fd in
-//   close fd
+let test (s : string) : IODiv unit (requires True) (ensures fun _ -> True)
+by (
+  explode () ;
+  bump_nth 3 ;
+  squash_intro () ;
+  explode ()
+)
+= let fd = open_file s in
+  let msg = read fd in
+  close fd
+
+let test_ (s : string) : IODiv unit (requires True) (ensures fun r -> terminates r /\ (exists fd msg. ret_trace r == [ EOpenfile s fd ; ERead fd msg ; EClose fd () ]))
+by (
+  explode ()
+)
+=
+  let fd = open_file s in
+  let msg = read fd in
+  close fd
 
 let test'' (fd : file_descr) : IODiv unit (requires True) (ensures fun _ -> True) =
   let msg = read fd in
@@ -1115,13 +1129,24 @@ let test'' (fd : file_descr) : IODiv unit (requires True) (ensures fun _ -> True
 let test_more (fd : file_descr) : IODiv unit (requires True) (ensures fun _ -> True) =
   test'' fd ; test'' fd
 
-let test_more' (fd : file_descr) : IODiv unit (requires True) (ensures fun _ -> True) =
-  // assume (forall (w1 w2 : twp unit). w1 `stronger_twp` w2) ;
-  // assume (forall (w : twp unit). (fun p -> True /\ (forall x. (fun _ -> True) x ==> p x)) `stronger_twp` w) ;
-  // assume (forall (w : twp unit) (wf : unit -> twp unit). (fun p -> True /\ (forall x. (fun _ -> True) x ==> p x)) `stronger_twp` wbind w wf) ;
-  assume (forall (wf : unit -> twp unit). (fun p -> True /\ (forall x. (fun _ -> True) x ==> p x)) `stronger_twp` wbind (fun p -> True /\ (forall x. (fun _ -> True) x ==> p x)) wf) ; // Enough, note it's wbind and not pwbind
-  // assume ((fun p -> True /\ (forall x. (fun _ -> True) x ==> p x)) `stronger_twp` wbind #unit #unit (fun p -> True /\ (forall x. (fun _ -> True) x ==> p x)) (fun (x : unit) -> (fun p -> True /\ (forall x. (fun _ -> True) x ==> p x)))) ; // Not that one
-  test'' fd ;
+// let test_more' (fd : file_descr) : IODiv unit (requires True) (ensures fun _ -> True) =
+//   // assume (forall (w1 w2 : twp unit). w1 `stronger_twp` w2) ;
+//   // assume (forall (w : twp unit). (fun p -> True /\ (forall x. (fun _ -> True) x ==> p x)) `stronger_twp` w) ;
+//   // assume (forall (w : twp unit) (wf : unit -> twp unit). (fun p -> True /\ (forall x. (fun _ -> True) x ==> p x)) `stronger_twp` wbind w wf) ;
+//   assume (forall (wf : unit -> twp unit). (fun p -> True /\ (forall x. (fun _ -> True) x ==> p x)) `stronger_twp` wbind (fun p -> True /\ (forall x. (fun _ -> True) x ==> p x)) wf) ; // Enough, note it's wbind and not pwbind
+//   // assume ((fun p -> True /\ (forall x. (fun _ -> True) x ==> p x)) `stronger_twp` wbind #unit #unit (fun p -> True /\ (forall x. (fun _ -> True) x ==> p x)) (fun (x : unit) -> (fun p -> True /\ (forall x. (fun _ -> True) x ==> p x)))) ; // Not that one
+//   test'' fd ;
+//   test'' fd ;
+//   test'' fd
+
+let test_more' (fd : file_descr) : IODiv unit (requires True) (ensures fun _ -> True)
+by (
+  explode () ;
+  bump_nth 3 ;
+  squash_intro () ;
+  explode ()
+)
+= test'' fd ;
   test'' fd ;
   test'' fd
 
@@ -1129,22 +1154,33 @@ let test3 (fd : file_descr) : IODiv unit (requires True) (ensures fun _ -> True)
   let msg = read fd in
   () ; () ; ()
 
-// let test' (s : string) : IODiv unit (requires True) (ensures fun _ -> True) =
-//   let fd = open_file s in
-//   let msg = read fd in
-//   ()
+let test' (s : string) : IODiv unit (requires True) (ensures fun _ -> True)
+by (
+  explode () ;
+  bump_nth 4 ;
+  squash_intro () ;
+  explode ()
+)
+= let fd = open_file s in
+  let msg = read fd in
+  ()
 
-let test' (s : string) : IODiv string (requires True) (ensures fun _ -> True) =
+let test'_ (s : string) : IODiv string (requires True) (ensures fun _ -> True) =
   let fd = open_file s in
   read fd
 
-// Somehow this one is ok though...
 let open_close_test (s : string) : IODiv unit (requires True) (ensures fun r -> terminates r /\ (exists fd. ret_trace r == [ EOpenfile s fd ; EClose fd () ])) =
   let fd = open_file s in
   close fd
 
-// let many_open_test (s : string) : IODiv unit (requires True) (ensures fun r -> terminates r) =
-//   let x = open_file s in
+// let many_open_test (s : string) : IODiv unit (requires True) (ensures fun r -> terminates r)
+// by (
+//   explode () ;
+//   bump_nth 5 ;
+//   squash_intro () ;
+//   dump "hhop"
+// )
+// = let x = open_file s in
 //   let y = open_file s in
 //   ()
 
